Add soundess statement for annotated checking

sandbox/Annotate.v
@@ -16,6 +16,8 @@ Inductive Term {Vs : Set} : Set :=
 Arguments Term : default implicits.
 Hint Constructors Term.
 
+Definition term_le {Vs : Set} : relation (Term Vs). Admitted.
+
 Inductive normal {Vs : Set} : Term Vs -> Prop :=
   | normal_bot : normal term_bot
   | normal_join x y : normal x -> normal y -> normal (term_join x y)
@@ -38,11 +40,43 @@ Hint Constructors Normal Inert.
 Arguments Normal : default implicits.
 Arguments Inert : default implicits.
 
+Fixpoint eval_normal {Vs : Set} (x : Normal Vs) : Term Vs :=
+  match x with
+  | Normal_bot => term_bot
+  | Normal_join x1 x2 => term_join (eval_normal x1) (eval_normal x2)
+  | Normal_inert i => eval_inert i
+  | Normal_lambda x1 => term_lambda (eval_normal x1)
+  end
+with eval_inert {Vs : Set} (x : Inert Vs) : Term Vs :=
+  match x with
+  | Inert_app x1 x2 => term_app (eval_inert x1) (eval_normal x2)
+  | Inert_var v => term_var v
+  end.
+
+Fixpoint
+  eval_normal_normal (Vs : Set) (n : Normal Vs) : normal (eval_normal n)
+with
+  eval_inert_inert (Vs : Set) (i : Inert Vs) : inert (eval_inert i).
+Proof.
+  induction n; simpl; auto.
+  induction i; simpl; auto.
+Qed.
+
 Inductive Tp {Vs : Set} : Set :=
   | Tp_var : Vs -> Tp
-  | Tp_exp : Tp -> Tp -> Tp.
+  | Tp_exp : Tp -> Tp -> Tp
+  (* TODO allow constants like [I] and [bool] *)
+.
 Hint Constructors Tp.
 Arguments Tp : default implicits.
+
+Definition A {Vs : Set} : Term Vs. Admitted.
+
+Fixpoint eval_type {Ts Vs : Set} (a : Tp Ts) : Term Vs :=
+  match a with
+  | Tp_var v => (* TODO *) term_bot
+  | Tp_exp a b => (* TODO *) term_bot
+  end.
 
 (* annotated normal forms *)
 Inductive TNormal {Vs Ts : Set} : Set :=
@@ -59,13 +93,28 @@ Hint Constructors TNormal TInert.
 Arguments TNormal : default implicits.
 Arguments TInert : default implicits.
 
+Fixpoint eval_tnormal {Vs Ts : Set} (x : TNormal Vs Ts) : Term Vs :=
+  match x with
+  | TNormal_bot => term_bot
+  | TNormal_join x1 x2 => term_join (eval_tnormal x1) (eval_tnormal x2)
+  | TNormal_inert i => eval_tinert i
+  | TNormal_lambda x1 => term_lambda (eval_tnormal x1)
+  | TNormal_ann a x1 => term_app (eval_type a) (eval_tnormal x1)
+  end
+with eval_tinert {Vs Ts : Set} (x : TInert Vs Ts) : Term Vs :=
+  match x with
+  | TInert_app x1 x2 => term_app (eval_tinert x1) (eval_tnormal x2)
+  | TInert_var v => term_var v
+  | TInert_ann a1 x1 => term_app (eval_type a1) (eval_tinert x1)
+  end.
+
 Fixpoint ann_lambda {Vs Ts : Set} (a : Tp Ts) (x : TNormal (option Vs) Ts) :
   TNormal (option Vs) Ts :=
   match x with
   | TNormal_bot => TNormal_bot
   | TNormal_join x1 x2 => TNormal_join (ann_lambda a x1) (ann_lambda a x2)
   | TNormal_inert i => TNormal_inert (ann_lambda' a i)
-  | TNormal_lambda v => (* TODO use option_map *) TNormal_bot
+  | TNormal_lambda x1 => (* TODO use option_map *) TNormal_bot
   | TNormal_ann a1 x1 => TNormal_ann a1 (ann_lambda a x1)
   end
 with ann_lambda' {Vs Ts : Set} (a : Tp Ts) (x : TInert (option Vs) Ts) :
@@ -77,32 +126,99 @@ with ann_lambda' {Vs Ts : Set} (a : Tp Ts) (x : TInert (option Vs) Ts) :
   | TInert_ann a1 x1 => TInert_ann a1 (ann_lambda' a x1)
   end.
 
-Inductive check {Vs Ts : Set} : relation (TNormal Ts Vs) :=
-  | check_refl x : check x x
-  | check_trans x y z : check x y -> check y z -> check x z
-  | check_bot x : check x TNormal_bot
-  | check_join_left x y : check (TNormal_join x y) x
-  | check_join_right x y : check (TNormal_join x y) y
+Inductive checks {Vs Ts : Set} : relation (TNormal Ts Vs) :=
+  | checks_refl x : checks x x
+  | checks_trans x y z : checks x y -> checks y z -> checks x z
+  | checks_bot x : checks x TNormal_bot
+  | checks_join_left x y : checks (TNormal_join x y) x
+  | checks_join_right x y : checks (TNormal_join x y) y
   (* ...app etc... *)
-  | check_expand_lambda a b x :
-      check (TNormal_ann (Tp_exp a b) (TNormal_lambda x))
+  | checks_expand_lambda a b x :
+      checks (TNormal_ann (Tp_exp a b) (TNormal_lambda x))
             (TNormal_lambda (TNormal_ann b (ann_lambda a x)))
-
-  | check_expand_join a x y :
-      check (TNormal_ann a (TNormal_join x y))
+  | checks_expand_join a x y :
+      checks (TNormal_ann a (TNormal_join x y))
             (TNormal_join (TNormal_ann a x) (TNormal_ann a y))
   (* TODO
   (* How to deal with covariance vs contravariance? *)
-  | check_eta_expand :
-  | check_conjugate :
-  | check_identity :
-  | check_clash_var_var :
-  | check_clash_var_exp :
-  | check_clash_exp_var :
+  | checks_eta_expand :
+  | checks_conjugate :
+  | checks_identity :
+  | checks_clash_var_var :
+  | checks_clash_var_exp :
+  | checks_clash_exp_var :
   *)
+with checks' {Vs Ts : Set} : relation (TInert Ts Vs) :=
+  (* TODO *)
 .
+
+Instance checks_sound (Vs Ts : Set) :
+  Proper (checks --> term_le) (@eval_tnormal Vs Ts).
+Proof.
+  intros y x xy; induction xy; simpl; auto.
+  - admit.
+  - admit.
+  - admit.
+  - admit.
+  - admit.
+  - admit.
+  - admit.
+Qed.
+
+Fixpoint check_step {Vs Ts : Set} (x : TNormal Ts Vs) :
+  option (TNormal Ts Vs) :=
+  match x with
+  (* TODO
+  | TNormal_bot => term_bot
+  | TNormal_join x1 x2 => term_join (eval_tnormal x1) (eval_tnormal x2)
+  | TNormal_inert i => eval_tinert i
+  | TNormal_lambda x1 => term_lambda (eval_tnormal x1)
+  | TNormal_ann a x1 => term_app (eval_type a) (eval_tnormal x1)
+  *)
+  | _ => None
+  end
+with check_step' {Vs Ts : Set} (x : TInert Vs Ts) :
+  option (TInert Vs Ts) :=
+  match x with
+  (* TODO
+  | TInert_app x1 x2 => term_app (eval_tinert x1) (eval_tnormal x2)
+  | TInert_var v => term_var v
+  | TInert_ann a1 x1 => term_app (eval_type a1) (eval_tinert x1)
+  *)
+  | _ => None
+  end.
+
+Fixpoint check_step_checks (Vs Ts : Set) (x : TNormal Vs Ts) :
+  match check_step x with
+  | None => True
+  | Some y => checks x y
+  end
+with check_step_checks' (Vs Ts : Set) (x : TInert Vs Ts) :
+  match check_step' x with
+  | None => True
+  | Some y => checks' x y
+  end.
+Proof.
+  - admit.
+  - admit.
+Admitted.
+
+Fixpoint try_check {Vs Ts : Set} (n : nat) (x : TNormal Vs Ts) :
+  option bool :=
+  match n with
+  | 0%nat => None
+  | Datatypes.S n' =>
+    match check_step x with
+    | Some x' => try_check n' x'
+    | None => (* TODO *) Some false
+    end
+  end.
+
+(* TODO
+Instance checks_complete (Vs Ts : Set) (x y : TNormal Vs Ts) : ???
+*)
 
 (* FIXME
 Definition fixes {Vs Ts : Set} (a : Tp Ts) (x : TNormal Ts Vs) : Prop :=
-  check (TNormal_ann a x) x.
+  checks (TNormal_ann a x) x.
 *)
